### $e^x$

 $$
\begin{align}
e^{x}&=1+x+\frac{x^{2}}{2}+\frac{x^{3}}{6} \\
&= 1+\sum_{k=1}^{\infty}  \frac{x^k}{k!} \quad \text{for } x \in \mathbb{R}
\end{align}
$$
### $\sin x$
$$
\begin{align}
\sin x &= x -\frac{x^{3}}{3}+\frac{x^{5}}{5}-\frac{x^{7}}{7} \\
&= \sum_{k=0}^{\infty} (-1)^{k} \frac{x^{2k+1}}{(2k + 1)!} \quad \text{for } x \in \mathbb{R}
\end{align}
$$
### $\cos x$
 $$
\begin{align}
\cos x&=1-\frac{x^{2}}{2!}+\frac{x^{4}}{4!} - \frac{x^{6}}{6!}\\
&= 1+\sum_{k=1}^{\infty} (-1)^{k} \frac{x^{2k}}{(2k)!} \quad \text{for } x \in \mathbb{R}
\end{align}
$$
### $\arctan x$

$$
\begin{align}
\arctan x &= x - \frac{x^{3}}{3}+\frac{x^{5}}{5}-\frac{x^{7}}{7} \\
&= \sum_{k=0}^{\infty} (-1)^{k} \frac{x^{2k+1}}{2k + 1} \quad \text{for } |x| \le 1
\end{align}
$$


### $\ln(x+1)$
$$
\begin{align}
\ln(1+x) &=x-\frac{x^{2}}{2}+\frac{x^{4}}{4} - \frac{x^{6}}{6}\\
&= \sum_{k=0}^{\infty} (-1)^{k} \frac{x^{k+1}}{k+1} \quad \text{for } -1 \lt x \le 1
\end{align}

$$

### $(1+x)^{p}$

$$
\begin{align}
(1+x)^{p} = \sum_{k=0}^{\infty} \frac{p(p-1)\dots(p-k+1)}{k!}x^{k}  \\
\text{for } p \in \mathbb{R} \text{ and } |x|\lt 1
\end{align}

$$
