$$
\begin{align}
& \frac{\mathrm{d}}{\mathrm{d}x}\sin (f(x)) = \cos x\cdot f'(x) \quad \text{(via chain rule)}\\ \\
& \frac{\mathrm{d}}{\mathrm{d}x}\cos (f(x)) = -\sin x \cdot f'(x)\quad \text{(via chain rule)} \\ \\ \\ \\
& \frac{\mathrm{d}}{\mathrm{d}x}\sec (f(x)) = \sec x\cdot \tan x\cdot f'(x) \quad \text{(via chain rule)}\\ \\
& \frac{\mathrm{d}}{\mathrm{d}x}\csc  (f(x)) = -\csc x\cdot \cot x \cdot f'(x)\quad \text{(via chain rule)} \\ \\ \\ \\
& \frac{\mathrm{d}}{\mathrm{d}x}\tan x=\frac{\sin x}{\cos x} = \frac{1}{\cos^2}=\sec^2x \quad \text{(via quotient rule)} \\ \\
& \frac{\mathrm{d}}{\mathrm{d}x}\tan f(x)=\sec^2x\cdot f'(x) \quad \text{(via chain rule)} \\ \\ 
& \frac{\mathrm{d}}{\mathrm{d}x}\cot f(x)=-\csc^2x\cdot f'(x) \quad \text{(via chain rule)} \\
\end{align}
$$

