$cis\theta$ is defined as being the sum of $\cos \theta$ and  $i\sin \theta$
$$cis\theta = \cos \theta + i \sin \theta$$

### Properties
$$\begin{array}{l}
1. \ cis\theta \cdot cis\phi = cis(\theta + \phi) \\ \\
2. \frac{cis\theta}{cis\phi} = cis(\theta - \phi) \\ \\
3. cis(\theta + k2\pi) = cis\theta, \quad \text{for all} \ k \in \mathbb{Z}
\end{array}
$$

> [!Tip] $\overline{z}$ has the same length as $z$ but argument of opposite direction
> $$\overline{z} = |z|cis(-\theta)$$

> [!Example] If $z=rcis\theta$, write $-iz$ in polar form
> $$-iz=cis(-\frac{\pi}{2})\cdot rcis\theta = rcis(\theta-\frac{\pi}{2})$$
