> **The Explicit formula**
> $u_n = u_1\cdot r^{n-1}$, where $u_1$ is the first term and $r$ is the common ratio

> **The Recursive formula**
> $u_n = u_{n-1}\cdot r$

When analyzing growth and decay it is common to have the initial condition correspond to zero, therefore the formula we apply is $u_n=u_0\cdot r^n$

If we are given an interest rate and inflation rate, we can find the true value of an investment by $$\text{real value} = \frac{\text{invested amount}\cdot\text{interest rate}}{\text{inflation rate}}$$
