The law is *universal* because the force of gravity acts between all masses. 

$F$ is the force of gravity acting between two point masses $(m_{1}, m_{2})$
$$
\begin{align}
&F\propto (m_{1}\cdot m_{2}) \\
&F\propto \frac{1}{r^2}
\end{align}
$$
Putting a constant of proportionality, $G=6.67\cdot 10^{-11}\mathrm{Nm}^2\mathrm{kg}^{-2}$ we get Newtons Universal Law Of Gravitation, which obeys the [[Inverse Square Law]]

$$
F=G \frac{m_{1}m_{2}}{r^{2}}
$$
> [!Tip] Newton's law is consistent with [[Kepler's Laws of Planetary Motion|Kepler's Third Law]]
>For circular gravitational orbits, the necessary [[centripetal force]] is provided by gravity
>$$
\begin{align}
&F_{\text{centripetal}}=F_{gravitational} \\
&\frac{mv^2}{r}=G \frac{Mm}{r^2} \\
&v^2=\frac{GM}{r} \\
 \\
& \text{then, since } v=\frac{2\pi r}{T} \\
& \left( \frac{2\pi r}{T} \right)^2 = \frac{GM}{r} \implies \\
&\frac{r^3}{T^2}=\frac{GM}{4\pi^2} \quad \text{(a constant)}
\end{align}
$$

> [!Example] Deriving Free Fall Acceleration 
> We know from [[Newton's Laws of Motion]] that $a=\frac{F}{m}$, where $m$ is relatively insignificant (because if it were significant, it would have a substantial gravitational field of its own)
> $$
g=\frac{F}{m}=\frac{\frac{GMm}{r^2}}{m}=\frac{GM}{r^2}
$$

An understanding of gravity enables us to model [[orbital motion]]